Started with example for polymorphic apply.

examples/PolyApply/MSimpleFunc.v
@@ -1,8 +1,16 @@
 Require Import ExtLib.Data.PList.
 
+Require Import MirrorCore.Lambda.Expr.
+Require Import MirrorCore.Simple.
 Require Import MirrorCore.Lib.ListView.
 Require Import MirrorCore.Lib.NatView.
+Require Import MirrorCore.Views.ViewSumN.
 Require Import MirrorCore.syms.SymOneOf.
+Require Import MirrorCore.syms.SymEnv.
+Require Import MirrorCore.Subst.FMapSubst.
+Require Import MirrorCore.Reify.Reify.
+Require Import MirrorCore.Reify.ReifyClass.
+Require Import MirrorCore.Reify.ReifyView.
 
 Require Import McExamples.PolyApply.MSimpleType.
 
@@ -11,5 +19,100 @@ Import OneOfType.
 Definition func_map : 
   OneOfType.pmap :=
   list_to_pmap
-    (pcons natFunc
-           (pcons (list_func typ) pnil)).
+    (pcons SymEnv.func
+           (pcons (natFunc:Type)
+                  (pcons (list_func typ) pnil))).
+
+Definition func := OneOfType.OneOf func_map.
+
+Global Instance TableView_func : PartialView func SymEnv.func :=
+  PartialViewPMap 1 func_map eq_refl.
+Global Instance NatView_func : PartialView func natFunc :=
+  PartialViewPMap 2 func_map eq_refl.
+Global Instance ListView_func : PartialView func (list_func typ) :=
+  PartialViewPMap 3 func_map eq_refl.
+
+Class Environment := { simple_env :> @SymEnv.functions typ _}.
+
+Existing Instance RelDec_from_RType.
+
+Section SimpleFunc.
+
+  Context {fs : Environment}.
+
+  Global Instance RSym_func : RSym func.
+  Proof.
+    apply RSymOneOf.
+    repeat first [eapply RSym_All_Branch_None | 
+                  eapply RSym_All_Branch_Some |
+                  eapply RSym_All_Empty].
+    
+    apply RSym_func; apply fs.
+    apply RSym_NatFunc.
+    apply RSym_ListFunc.
+  Defined.
+
+  Global Instance RSymOk_func : RSymOk RSym_func.
+  apply RSymOk_OneOf.
+
+  repeat first [eapply RSymOk_All_Branch_None | 
+                eapply RSymOk_All_Branch_Some; [apply _ | |] |
+                eapply RSymOk_All_Empty]. 
+  Defined.
+
+  Global Instance Expr_expr : ExprI.Expr _ (expr typ func) := @Expr_expr typ func _ _ _.
+  Global Instance Expr_ok : @ExprI.ExprOk typ RType_typ (expr typ func) Expr_expr := @ExprOk_expr _ _ _ _ _ _ _ _.
+
+  Require Import MirrorCore.VariablesI.
+  Require Import MirrorCore.Lambda.ExprVariables.
+
+  Global Instance ExprVar_expr : ExprVar (expr typ func) := _.
+  Global Instance ExprVarOk_expr : ExprVarOk ExprVar_expr := _.
+
+  Global Instance ExprUVar_expr : ExprUVar (expr typ func) := _.
+  Global Instance ExprUVarOk_expr : ExprUVarOk ExprUVar_expr := _.
+
+  Definition subst : Type :=
+    FMapSubst.SUBST.raw (expr typ func).
+  Global Instance SS : SubstI.Subst subst (expr typ func) :=
+    @FMapSubst.SUBST.Subst_subst _.
+  Global Instance SU : SubstI.SubstUpdate subst (expr typ func) :=
+    @FMapSubst.SUBST.SubstUpdate_subst _ _ _ _.
+Check SubstI.SubstOk.
+  Global Instance SO : @SubstI.SubstOk _ _ _ _ _ SS :=
+    @FMapSubst.SUBST.SubstOk_subst typ RType_typ (expr typ func) _.
+  Global Instance SUO : @SubstI.SubstUpdateOk _ _ _ _ _ _ SU SO :=  @FMapSubst.SUBST.SubstUpdateOk_subst typ RType_typ (expr typ func) _ _.
+
+End SimpleFunc.
+
+Section ReifyFunc.
+
+  Global Instance Reify_func : Reify (expr typ func) :=
+    Reify_func typ func (reify_nat typ func :: reify_list typ func :: nil).
+
+End ReifyFunc.
+
+Definition rt := reify_scheme typ.
+Definition re := reify_scheme (expr typ func).
+
+Reify Declare Syntax patterns_simple_typ := rt.
+(*
+Gregory, the next line does not work.
+
+Reify Declare Syntax patterns_simple_expr := re.
+*)
+
+
+Ltac reify trm :=
+  let t := fresh "t" in
+  let k e := pose e as t
+  in
+  reify_expr patterns_simple_typ k [[ True ]] [[ trm ]]; cbv beta iota in t.
+
+Goal True.
+  reify nat.
+  reify (list nat).
+  reify (list (list nat)).
+  
+  apply I.
+Qed.
