examples/PolyApply/MSimpleType.v
@@ -11,24 +11,26 @@ Require Import MirrorCore.ExprI.
 Require Import MirrorCore.TypesI.
 Require Import MirrorCore.SymI.
 Require Import MirrorCore.MTypes.ModularTypes.
-Require Import MirrorCore.syms.SymOneOf.
+Require Import MirrorCore.MTypes.TSymOneOf.
 Require Import MirrorCore.Lambda.Ptrns.
 Require Import MirrorCore.MTypes.ListType.
 Require Import MirrorCore.MTypes.BaseType.
 Require Import MirrorCore.Views.ViewSumN.
+Require Import MirrorCore.Reify.ReifyClass.
+Require Import MirrorCore.Reify.ReifyView.
 
 Set Implicit Arguments.
 Set Strict Implicit.
 
 Import OneOfType.
 
-Definition typ_map x := 
+Definition typ_map := 
   list_to_pmap
-    (pcons (base_typ x)
-           (pcons (list_typ x)
+    (pcons base_typ
+           (pcons list_typ
                   pnil)).
 
-Definition typ' x := OneOf (typ_map x).
+Definition typ' := OneOfF typ_map.
 
 Definition typ := mtyp typ'.
 
@@ -50,7 +52,7 @@ Proof.
   intros.
   destruct a as [a1 v1].
   destruct b as [a2 v2].
-  unfold typ_map, list_to_pmap in *. simpl in *.
+  unfold typ_map, list_to_pmap, type_nth in *; simpl in *.
   pmap_lookup'_simpl; try eq_dec_right.  
   pose proof (list_typ_dec v1 v2).
   destruct H; [left; subst; reflexivity|].
@@ -64,18 +66,19 @@ Defined.
 
 Definition typ'D {n} (t : typ' n) : type_for_arity n.
 Proof.
-  unfold typ', typ_map, list_to_pmap in t; simpl in t.
+  unfold typ', typ_map, list_to_pmap, type_nth in t; simpl in t.
   destruct t as [p v].
+  unfold type_nth in v.
   pmap_lookup'_simpl.
   apply list_typD; assumption.
   apply base_typD; assumption.
 Defined.
 
 Global Instance TypeView_list_typ' : PartialView (typ' 1) (list_typ 1) :=
-  PartialViewPMap 2 (typ_map 1) eq_refl.
+  PartialViewPMap_Type 2 (typ_map) eq_refl 1.
   
 Global Instance TypeView_base_typ' : PartialView (typ' 0) (base_typ 0) :=
-  PartialViewPMap 1 (typ_map 0) eq_refl.
+  PartialViewPMap_Type 1 typ_map eq_refl 0.
   
 Instance TypeView_list_typ : PartialView typ (list_typ 1 * typ).
 eapply PartialView_trans. 
@@ -89,4 +92,49 @@ eapply TypeView_sym0.
 apply TypeView_base_typ'.
 Defined.
 
+Definition TSymAll_typ_map : TSym_All typ_map.
+  repeat first [eapply TSym_All_Branch_None |
+                eapply TSym_All_Branch_Some; [eapply _ | |] |
+                eapply TSym_All_Empty].
+Defined.
+
+Global Instance TSym_typ' : TSym typ'.
+  apply TSymOneOf. apply TSymAll_typ_map.
+Defined.
+
+
+Global Instance RType_typ : RType typ.
+apply RType_mtyp. 
+apply _.
+Defined.
+
+Global Instance RTypeOk_typ : RTypeOk.
+apply RTypeOk_mtyp.
+Defined.
+
+Global Instance Typ2_tyArr : Typ2 RType_typ Fun := Typ2_Fun.
+Global Instance Typ2Ok_tyArr : Typ2Ok Typ2_tyArr := Typ2Ok_Fun.
+
+Global Instance Typ0_tyProp : Typ0 RType_typ Prop := Typ0_sym tyProp.
+Global Instance Typ0Ok_tyProp : Typ0Ok Typ0_tyProp := Typ0Ok_sym tyProp.
+
+Global Instance Typ0_tyNat : Typ0 RType_typ nat := Typ0_sym tyNat.
+Global Instance Typ0Ok_tyNat : Typ0Ok Typ0_tyNat := Typ0Ok_sym tyNat.
+
+Global Instance Typ0_tyString : Typ0 RType_typ String.string := Typ0_sym tyString.
+Global Instance Typ0Ok_tyString : Typ0Ok Typ0_tyString := Typ0Ok_sym tyString.
+
+Global Instance Typ0_tyBool : Typ0 RType_typ bool := Typ0_sym tyBool.
+Global Instance Typ0Ok_tyBool : Typ0Ok Typ0_tyBool := Typ0Ok_sym tyBool.
+
+Global Instance Typ1_tyList : Typ1 RType_typ list := Typ1_sym (f_insert tList).
+Global Instance Typ1Ok_tyList : Typ1Ok Typ1_tyList := Typ1Ok_sym (f_insert tList).
+
+Section ReifyType.
+
+Global Instance Reify_typ : Reify typ := 
+  Reify_typ typ (reify_base_typ typ ::
+                 reify_list_typ typ :: nil).
+
+End ReifyType.
 
